lean/src/gdt/a_eval_theorem.lean
@@ -1,0 +1,11 @@
+import .defs
+
+variable [GuardModule]
+open GuardModule
+
+-- 𝒜 maintains semantics
+-- This theorem implies that ant_eval returns a list of length at most 1.
+-- This means that the refinement types created by 𝒜 are disjoint.
+theorem 𝒜_eval :
+    ∀ env: Env, ∀ gdt: Gdt,
+        (option_to_list $ gdt_eval gdt env) = ant_eval (𝒜 gdt) env := sorry
