lean/src/gdt/defs.lean
@@ -1,8 +1,6 @@
 -- # Abstract Guard Trees
 -- This chapter covers basic guard trees with abstract guards.
 
-namespace gdt
-
 class GuardModule :=
     -- Represents the type of all guards.
     (Grd : Type)
@@ -103,8 +101,6 @@ def 𝒰_acc : Φ → Gdt → Φ
 def 𝒰 : Gdt → Φ := 𝒰_acc Φ.true
 
 
--- ### start: optional
-
 -- Alternative definition without accumulator
 def 𝒰' : Gdt → Φ
 | (Gdt.leaf _) := Φ.false
@@ -112,143 +108,6 @@ def 𝒰' : Gdt → Φ
 | (Gdt.grd grd tree) := Φ.or
             (Φ.negGrd grd)
             (Φ.and (Φ.grd grd) (𝒰' tree))
-
-
-lemma Φ_true_and (ty: Φ): Φ_eval (Φ.true.and ty) = Φ_eval ty :=
-begin
-    funext env,
-    unfold Φ_eval
-end
-
-
-lemma Φ_false_and (ty: Φ): Φ_eval Φ.false = Φ_eval (ty.and Φ.false) :=
-begin
-    funext env,
-    unfold Φ_eval,
-    cases (Φ_eval ty env),
-    repeat { unfold Φ_eval._match_3 }
-end
-
-lemma Φ_and_assoc (ty1: Φ) (ty2: Φ) (ty3: Φ):
-    Φ_eval ((ty1.and ty2).and ty3) = Φ_eval (ty1.and (ty2.and ty3)) :=
-begin
-    funext env,
-    rw Φ_eval,
-    
-    simp,
-    cases h: (Φ_eval (ty1.and ty2) env),
-    repeat {
-        rw Φ_eval,
-        simp,
-        rw Φ_eval at h,
-        simp at h,
-        cases h2: (Φ_eval ty1 env),
-        repeat {
-            rw Φ_eval._match_3,
-        },
-    },
-    
-    repeat {
-        rw h2 at h,
-        rw Φ_eval._match_3 at h,
-    },
-
-    case option.none option.some {
-        rw Φ_eval, simp,
-        rw h,
-        rw Φ_eval._match_3, 
-    },
-    
-    case option.some option.none {
-        cc,
-    },
-
-    case option.some option.some {
-        rw Φ_eval, simp, rw h,
-        rw Φ_eval._match_3,
-    }
-end
-
-lemma Φ_and_or_distrib (ty1: Φ) (ty2: Φ) (ty3: Φ):
-    Φ_eval ((ty1.and ty2).or (ty1.and ty3)) = Φ_eval (ty1.and (ty2.or ty3)) :=
-begin
-    funext env,
-    unfold Φ_eval, simp,
-    cases (Φ_eval ty1 env),
-        unfold Φ_eval._match_3,
-        unfold Φ_eval._match_2,
-
-        unfold Φ_eval._match_3,
-end
-
-lemma rw_right_or (ty1: Φ) (ty2: Φ) (ty3: Φ):
-    (Φ_eval ty2 = Φ_eval ty3)
-    → (Φ_eval (ty1.or ty2) = Φ_eval (ty1.or ty3)) :=
-begin
-    assume h,
-    funext env,
-    rw Φ_eval,
-    rw Φ_eval,
-    rw h,
-end
-
-
-lemma 𝒰_𝒰'_equiv' (acc: Φ) (gdt: Gdt) :
-    Φ_eval (𝒰_acc acc gdt) = Φ_eval (Φ.and acc (𝒰' gdt)) :=
-begin
-    funext env,
-    induction gdt generalizing acc,
-
-    -- case leaf
-    unfold 𝒰_acc,
-    unfold 𝒰',
-    rw Φ_false_and,
-
-    -- case branch
-    
-    unfold 𝒰_acc,
-    rw gdt_ih_a_1,
-    rw Φ_eval,
-    rw gdt_ih_a,
-    rw← Φ_eval,
-    unfold 𝒰',
-    rw Φ_and_assoc,
-
-    -- case grd
-    rw 𝒰',
-
-    rw 𝒰_acc,
-    
-    rw Φ_eval,
-    rw Φ_eval,
-    rw gdt_ih,
-    rw ←Φ_eval,
-    rw ←Φ_eval,
-    rw rw_right_or,
-    rw Φ_and_or_distrib,
-    rw Φ_and_assoc,
-end
-
-
-lemma 𝒰_𝒰'_equiv : Φ_eval ∘ 𝒰 = Φ_eval ∘ 𝒰' := 
-begin
-    unfold function.comp,
-    funext x,
-    rw 𝒰,
-    rw ←Φ_true_and (𝒰' x),
-    rw 𝒰_𝒰'_equiv'
-end
-
--- ### end: optional
-
--- Uncovered refinement types capture all values that are not covered.
--- This theorem might be easier to show for 𝒰' rather than 𝒰.
-theorem 𝒰_eval :
-    ∀ env: Env, ∀ gdt: Gdt,
-        (gdt_eval gdt env ≠ none) ↔ (Φ_eval (𝒰 gdt) env = none)
-    := sorry
-
-
 
 -- ## Annotate
 
@@ -276,12 +135,3 @@ def ant_eval : Ant → Env → list (Env × Leaf)
 def option_to_list { α: Type _ } : option α → list α
 | none := []
 | (some val) := [val]
-
--- 𝒜 maintains semantics
--- This theorem implies that ant_eval returns a list of length at most 1.
--- This means that the refinement types created by 𝒜 are disjoint.
-theorem 𝒜_eval :
-    ∀ env: Env, ∀ gdt: Gdt,
-        (option_to_list $ gdt_eval gdt env) = ant_eval (𝒜 gdt) env := sorry
-
-end gdt
