lean/src/gdt/lemmas.lean
@@ -1,0 +1,130 @@
+import .defs
+
+variable [GuardModule]
+open GuardModule
+
+lemma Φ_true_and (ty: Φ): Φ_eval (Φ.true.and ty) = Φ_eval ty :=
+begin
+    funext env,
+    unfold Φ_eval
+end
+
+
+lemma Φ_false_and (ty: Φ): Φ_eval Φ.false = Φ_eval (ty.and Φ.false) :=
+begin
+    funext env,
+    unfold Φ_eval,
+    cases (Φ_eval ty env),
+    repeat { unfold Φ_eval._match_3 }
+end
+
+lemma Φ_and_assoc (ty1: Φ) (ty2: Φ) (ty3: Φ):
+    Φ_eval ((ty1.and ty2).and ty3) = Φ_eval (ty1.and (ty2.and ty3)) :=
+begin
+    funext env,
+    rw Φ_eval,
+    
+    simp,
+    cases h: (Φ_eval (ty1.and ty2) env),
+    repeat {
+        rw Φ_eval,
+        simp,
+        rw Φ_eval at h,
+        simp at h,
+        cases h2: (Φ_eval ty1 env),
+        repeat {
+            rw Φ_eval._match_3,
+        },
+    },
+    
+    repeat {
+        rw h2 at h,
+        rw Φ_eval._match_3 at h,
+    },
+
+    case option.none option.some {
+        rw Φ_eval, simp,
+        rw h,
+        rw Φ_eval._match_3, 
+    },
+    
+    case option.some option.none {
+        cc,
+    },
+
+    case option.some option.some {
+        rw Φ_eval, simp, rw h,
+        rw Φ_eval._match_3,
+    }
+end
+
+lemma Φ_and_or_distrib (ty1: Φ) (ty2: Φ) (ty3: Φ):
+    Φ_eval ((ty1.and ty2).or (ty1.and ty3)) = Φ_eval (ty1.and (ty2.or ty3)) :=
+begin
+    funext env,
+    unfold Φ_eval, simp,
+    cases (Φ_eval ty1 env),
+        unfold Φ_eval._match_3,
+        unfold Φ_eval._match_2,
+
+        unfold Φ_eval._match_3,
+end
+
+lemma rw_right_or (ty1: Φ) (ty2: Φ) (ty3: Φ):
+    (Φ_eval ty2 = Φ_eval ty3)
+    → (Φ_eval (ty1.or ty2) = Φ_eval (ty1.or ty3)) :=
+begin
+    assume h,
+    funext env,
+    rw Φ_eval,
+    rw Φ_eval,
+    rw h,
+end
+
+
+lemma 𝒰_𝒰'_equiv' (acc: Φ) (gdt: Gdt) :
+    Φ_eval (𝒰_acc acc gdt) = Φ_eval (Φ.and acc (𝒰' gdt)) :=
+begin
+    funext env,
+    induction gdt generalizing acc,
+
+    -- case leaf
+    unfold 𝒰_acc,
+    unfold 𝒰',
+    rw Φ_false_and,
+
+    -- case branch
+    
+    unfold 𝒰_acc,
+    rw gdt_ih_a_1,
+    rw Φ_eval,
+    rw gdt_ih_a,
+    rw← Φ_eval,
+    unfold 𝒰',
+    rw Φ_and_assoc,
+
+    -- case grd
+    rw 𝒰',
+
+    rw 𝒰_acc,
+    
+    rw Φ_eval,
+    rw Φ_eval,
+    rw gdt_ih,
+    rw ←Φ_eval,
+    rw ←Φ_eval,
+    rw rw_right_or,
+    rw Φ_and_or_distrib,
+    rw Φ_and_assoc,
+end
+
+
+lemma 𝒰_𝒰'_equiv : Φ_eval ∘ 𝒰 = Φ_eval ∘ 𝒰' := 
+begin
+    unfold function.comp,
+    funext x,
+    rw 𝒰,
+    rw ←Φ_true_and (𝒰' x),
+    rw 𝒰_𝒰'_equiv'
+end
+
