lean/src/gdt/u_eval_theorem.lean
@@ -1,0 +1,12 @@
+import .defs
+
+variable [GuardModule]
+open GuardModule
+
+-- Uncovered refinement types capture all values that are not covered.
+-- This theorem might be easier to show for 𝒰' rather than 𝒰.
+theorem 𝒰_eval :
+    ∀ env: Env, ∀ gdt: Gdt,
+        (gdt_eval gdt env ≠ none) ↔ (Φ_eval (𝒰 gdt) env = none)
+    := sorry
+
