lean/src/main.lean
@@ -1,3 +1,9 @@
 
-import gdt
-import ngdt
+import .gdt.defs
+import .gdt.lemmas
+import .gdt.a_eval_theorem
+import .gdt.u_eval_theorem
+
+import .ngdt.defs
+import .ngdt.theorems
+
