lean/src/ngdt/theorems.lean
@@ -1,0 +1,33 @@
+import .defs
+variable [NGuardModule]
+open NGuardModule
+
+-- Reduction to Guard Trees maintains semantic.
+theorem ngdt_eval_eq_gdt_eval :
+        ngdt_eval = gdt_eval ∘ ngdt_to_gdt := sorry
+
+
+-- Every redundant leaf can be marked as inaccessible instead and
+-- every inaccessible leaf can be marked as accessible instead without invalidating the theorem. This only weakens the analysis.
+
+theorem main [decidable_eq Leaf] : ∀ ngdt: NGdt, ∀ is_empty: Gs,
+    (
+        let ⟨ a, i, r ⟩ := ℛ is_empty.val $ 𝒜 $ ngdt_to_gdt ngdt
+        in
+                -- leaves that are redundant and neither accessible nor inaccessible can be removed without changing semantics
+                ngdt_eval_option (remove_leaves ((r.remove_all i).remove_all a) ngdt)
+                = ngdt_eval ngdt
+            ∧ 
+                -- reachable leaves are accessible.
+                -- Since R is clearly a partition for disjoint leaves,
+                -- this also means that non-accessible leaves are unreachable.
+                ∀ env: Env,
+                    (match ngdt_eval ngdt env with
+                    | (some ⟨ _, NLeaf.leaf leaf ⟩) := leaf ∈ a
+                    | _ := true
+                    end : Prop)
+        : Prop
+    )
+    -- We probably need 𝒜_eval for proving this.
+    := sorry
+
